theories/Config.v
@@ -57,6 +57,18 @@ Section BackendConfig.
     eval_anf : bool;
   }.
 
+  Variant ASTType :=
+  | LambdaBox
+  | LambdaBoxTyped
+  | LambdaBoxMut   : certicoq_config -> ASTType
+  | LambdaBoxLocal : certicoq_config -> ASTType
+  | LambdaANF      : certicoq_config -> ASTType
+  | LambdaANFC     : certicoq_config -> ASTType.
+
+  Record ast_config := {
+    ast_type : ASTType;
+  }.
+
   Inductive backend_config :=
   | Rust   : rust_config -> backend_config
   | Elm    : elm_config -> backend_config
@@ -64,7 +76,8 @@ Section BackendConfig.
   | Wasm   : wasm_config -> backend_config
   | OCaml  : ocaml_config -> backend_config
   | CakeML : cakeml_config -> backend_config
-  | Eval   : eval_config -> backend_config.
+  | Eval   : eval_config -> backend_config
+  | AST    : ast_config -> backend_config.
 
 End BackendConfig.
 
