theories/backends/ASTBackend.v
@@ -1,0 +1,56 @@
+From MetaRocq.Utils Require Import utils.
+From MetaRocq.Utils Require Import bytestring.
+From MetaRocq.Erasure.Typed Require Import ResultMonad.
+From CertiCoq Require Import Compiler.pipeline.
+From CertiCoq Require Import Common.Pipeline_utils.
+From Peregrine Require Import Config.
+From Peregrine Require Import Utils.
+From Peregrine Require Import PAst.
+From Peregrine Require Import CertiCoqBackend.
+From ExtLib.Structures Require Import Monad.
+
+Import MonadNotation.
+
+Local Open Scope bs_scope.
+
+
+
+Definition default_ast_config := {|
+  ast_type := LambdaBox;
+|}.
+
+Definition default_ast_c_config := {|
+  direct    := true;
+  c_args    := 5;
+  o_level   := 0;
+  anf_conf  := 0;
+  prefix    := "";
+  body_name := "body";
+|}.
+
+Definition ast_phases := {|
+  implement_box_c  := Compatible false;
+  implement_lazy_c := Compatible false;
+  cofix_to_laxy_c  := Compatible false;
+  betared_c        := Compatible false;
+  unboxing_c       := Compatible false;
+  dearg_ctors_c    := Compatible false;
+  dearg_consts_c   := Compatible false;
+|}.
+
+
+
+Definition extract_ast (remaps : constant_remappings)
+                       (custom_attr : custom_attributes)
+                       (opts : ast_config)
+                       (file_name : string)
+                       (p : PAst.PAst)
+                       : result string string :=
+  match opts.(ast_type) with
+  | LambdaBox => Ok "TODO"
+  | LambdaBoxTyped => Ok "TODO"
+  | LambdaBoxMut c => Ok "TODO"
+  | LambdaBoxLocal c => Ok "TODO"
+  | LambdaANF c => Ok "TODO"
+  | LambdaANFC c => Ok "TODO"
+  end.
